This branch uses the tensor product permuting the vector to keep an ordered basis according to the variables order.

Q_State.thy
@@ -72,13 +72,6 @@ proof-
     unfolding set_vars_def by auto
 qed
 
-lemma "finite s \<Longrightarrow> x \<in> s \<Longrightarrow>
-       (ind_in_set s) x =  to_nat_set s x"
-  unfolding ind_in_set_def to_nat_set_def
-  
-  apply rule
-  sorry
-
   value "to_nat_set {0::nat, 1,2,8,10,15} ` {2,10}"
   value "ind_in_set {0::nat, 1,2,8,10,15} ` {2,10} "
 
@@ -97,7 +90,7 @@ definition lin_sets::"nat \<Rightarrow> 'q set \<Rightarrow> nat set"
 definition list_dims::"'q set \<Rightarrow> nat list"
   where "list_dims qvars \<equiv> replicate (card qvars) 2"
 
-definition dims :: "nat list \<Rightarrow> nat set \<Rightarrow> nat list" where
+definition dims :: "'a list \<Rightarrow> nat set \<Rightarrow> 'a list" where
   "dims tv vs = nths tv vs"
 
 \<comment>\<open> Lemmas on ptensor_vec \<close>
@@ -125,10 +118,26 @@ lemma digit_decode_non_vars:"digit_decode (nths (replicate (card d1) 2) (- {0..<
   using nths_set_gt_list_length
   by (metis digit_decode.simps(1) length_digit_encode length_replicate)
 
+lemma f1:"nths (digit_encode (nths (replicate (card d1) 2) d1) i) (- ind_in_set d1 ` d1) = []"
+proof -
+  have "length (nths (nths (replicate (card d1) 2) d1) (- ind_in_set d1 ` d1)) = 0"
+    using nths_reencode_eq_comp[of d1 d1 "(replicate (card d1) 2)",simplified] by auto    
+  then have 
+     "length (nths (digit_encode (nths (replicate (card d1) 2) d1) i) (- ind_in_set d1 ` d1)) = 0"    
+    by (simp add: length_digit_encode length_nths')           
+  then show ?thesis by auto
+qed
+
+lemma digit_decode_non_vars1:"digit_decode 
+    (nths (nths (replicate (card d1) 2) d1) (- ind_in_set d1 ` d1))
+    (nths (digit_encode (nths (replicate (card d1) 2) d1) i) (- ind_in_set d1 ` d1)) = 0"   
+  using f1
+  by (simp add: nths_reencode_eq_comp)
+
 lemma digit_decode_vars:
    "i< (2::nat) ^ card (d1) \<Longrightarrow> 
-    digit_decode (nths (replicate (card d1) 2) {0..<card d1})
-                 (nths (digit_encode (replicate (card d1) 2) i) {0..<card d1}) = i"  
+    digit_decode (nths (nths (replicate (card d1) 2) (d1 \<union> {})) (ind_in_set (d1 \<union> {}) ` d1))
+     (nths (digit_encode (nths (replicate (card d1) 2) (d1 \<union> {})) i) (ind_in_set (d1 \<union> {}) ` d1))  = i"  
   by (simp add: length_digit_encode nths_all)
   
 lemma list_of_neutral:"list_of_vec (vCons 1 vNil) = [1::'a::comm_ring_1]"
@@ -145,22 +154,27 @@ lemma idempoten_qstate1:
     a0:"dim_vec (v::('a::comm_ring_1) vec) = (2::nat) ^ card (d1)" and
     a1:"i < dim_vec v"
   shows 
-     "partial_state.tensor_vec (replicate (card d1) (2::nat))
-             {0::nat..<card  d1} v (vCons 1 vNil) $ i = 
+     "partial_state2.ptensor_vec (replicate (card d1) (2::nat))
+             d1 {} v (vCons 1 vNil) $ i = 
          v $ i"
 proof-
-  interpret ps2:partial_state "(replicate (card d1) (2::nat))" "{0::nat..<card  d1}" .
-  let  ?d0 = "digit_decode (nths (replicate (card d1) 2) (- {0..<card d1}))
-                  (nths (digit_encode (replicate (card d1) 2) i) (- {0..<card d1}))"
-  have vcons_0:"vCons 1 vNil $ ?d0 = 1" by  (auto simp add: digit_decode_non_vars)
-  moreover have  "digit_decode (nths (replicate (card d1) 2) {0..<card d1})
-                 (nths (digit_encode (replicate (card d1) 2) i) {0..<card d1}) = i" 
-    using digit_decode_vars a0 a1 by auto
-  moreover have " (prod_list (replicate (card d1) 2)) = (2::nat) ^ card (d1)" by auto
-  ultimately show ?thesis unfolding ps2.tensor_vec_def 
+  interpret ps2:partial_state2 "(replicate (card d1) (2::nat))" d1 "{}" apply standard by auto
+  let  ?d0 = "digit_decode (nths ps2.dims0 (- ps2.vars1'))
+                 (nths (digit_encode ps2.dims0 i) (- ps2.vars1'))"
+  have vcons_0:"vCons 1 vNil $ ?d0 = 1" unfolding ps2.dims0_def ps2.vars0_def ps2.vars1'_def 
+    by  (auto simp add: digit_decode_non_vars1)
+  moreover have  "digit_decode (nths ps2.dims0 ps2.vars1') (nths (digit_encode ps2.dims0 i) ps2.vars1') = i"
+    unfolding ps2.dims0_def ps2.vars0_def ps2.vars1'_def 
+    sorry
+  moreover have "prod_list (nths (replicate (card d1) 2) d1) = (2::nat) ^ card (d1)" 
+    sorry by auto
+  ultimately show ?thesis unfolding ps2.ptensor_vec_def 
       partial_state.tensor_vec_def state_sig.d_def partial_state.encode1_def 
-      partial_state.encode2_def partial_state.dims1_def partial_state.dims2_def     
-    using a1 a0   apply clarsimp  by (auto simp add: vcons_0)
+      partial_state.encode2_def partial_state.dims1_def partial_state.dims2_def ps2.dims0_def
+                                ps2.vars0_def                         
+    using a1 a0   apply clarsimp
+    using digit_decode_non_vars1 partial_state2.intro partial_state2.vars0_def partial_state2.vars1'_def 
+    by auto 
     
 qed
 
@@ -241,17 +255,17 @@ qed
 lemma idempoten_qstate:
   assumes 
     a1:"dim_vec (v::('a::comm_ring_1) vec) = (2::nat) ^ card d" and a2:"finite d"
-  shows "partial_state.tensor_vec (list_dims d)  {0::nat..<card d} v (vCons (1) vNil) = v"
+  shows "partial_state2.ptensor_vec (list_dims d)  d {} v (vCons (1) vNil) = v"
   unfolding list_dims_def
-  using idempoten_qstate1[OF a1] idempoten_qstate2[OF  a1 a2]
+  using idempoten_qstate1[OF a1] idempoten_qstate2[OF  a1 a2] sorry
   using a2 by blast
 
 
 definition mapping::"'q set \<Rightarrow> 'q set \<Rightarrow> nat set \<times> nat set"
   where "mapping s1 s2 \<equiv>({},{})"
 
-typedef (overloaded) ('q,'a::comm_ring_1)
-  QState = "{(s,v)| (s::'q set) (v::'a list).                                   
+typedef (overloaded) ('a::comm_ring_1)
+  QState = "{(s,v)| (s::nat set) (v::'a list).                                   
               length v = (2^(card s)) \<and> finite s \<and>
               (s = {} \<longrightarrow> ((v!0) = (1::'a)))}"
   morphisms uQState Abs_QState  
@@ -259,7 +273,7 @@ typedef (overloaded) ('q,'a::comm_ring_1)
 
 setup_lifting type_definition_QState
 
-definition tensor_mat_ord::"('q,'a)QState \<Rightarrow> 'q set \<Rightarrow> 'a::comm_ring_1 mat \<Rightarrow> ('q,'a)QState set"
+definition tensor_mat_ord::"'a QState \<Rightarrow> nat set \<Rightarrow> 'a::comm_ring_1 mat \<Rightarrow> 'a QState set"
   where "tensor_mat_ord Q q M \<equiv> {}"
 
 lemma QState_rel1:"length(snd(uQState x)) = 2 ^ card (fst(uQState x))"  
@@ -270,7 +284,7 @@ proof -
   then show ?thesis using uQState  by (auto simp add:  split_beta)    
 qed
 
-lemma QState_rel2:"fst (uQState (x::('q,'a::comm_ring_1) QState )) = {} \<longrightarrow> 
+lemma QState_rel2:"fst (uQState (x::('a::comm_ring_1) QState )) = {} \<longrightarrow> 
                   (((snd (uQState x)) ! 0) = 1)"
 proof -
   have "\<exists>B v. uQState x = (B, v) \<and> length v = (2 ^ card B) \<and> 
@@ -279,24 +293,24 @@ proof -
   then show ?thesis using uQState  by (auto simp add:  split_beta)       
 qed
 
-lemma QState_rel3:"finite (fst (uQState (x::('q,'a::comm_ring_1) QState )))"
+lemma QState_rel3:"finite (fst (uQState (x::('a::comm_ring_1) QState )))"
   apply transfer by auto
  
-lift_definition QState_vars :: "('q,'a::comm_ring_1) QState \<Rightarrow> 'q set" is fst .
-lift_definition QState_list :: "('q,'a::comm_ring_1) QState \<Rightarrow> 'a::comm_ring_1 list" is snd .
-lift_definition QState_vector::"('q,'a::comm_ring_1) QState \<Rightarrow> 'a::comm_ring_1 vec" is "\<lambda>s. vec_of_list (snd s)" .
-lift_definition QState :: "'q set \<times> 'a::comm_ring_1 list \<Rightarrow> ('q,'a)QState" is  
+lift_definition QState_vars :: "('a::comm_ring_1) QState \<Rightarrow> nat set" is fst .
+lift_definition QState_list :: "('a::comm_ring_1) QState \<Rightarrow> 'a::comm_ring_1 list" is snd .
+lift_definition QState_vector::"('a::comm_ring_1) QState \<Rightarrow> 'a::comm_ring_1 vec" is "\<lambda>s. vec_of_list (snd s)" .
+lift_definition QState :: "nat set \<times> 'a::comm_ring_1 list \<Rightarrow> 'a QState" is  
   "\<lambda>s. (if fst s = {} \<and> snd s = [1] then (fst s, snd s)
        else (if finite (fst s) \<and> fst s \<noteq> {} \<and> length (snd s) = 2 ^ (card (fst s)) then (fst s, snd s)
        else ({}, [1])))"  by auto
 
-lift_definition Conc :: " ('q,'a) QState \<Rightarrow> 'q set \<times> 'a::comm_ring_1 vec" is
+lift_definition Conc :: " 'a QState \<Rightarrow> nat set \<times> 'a::comm_ring_1 vec" is
   "\<lambda>s. (QState_vars s, QState_vector s)" .
 
 lemma uqstate_fst:"fst (uQState a) = QState_vars a" apply transfer' by auto
 lemma uqstate_snd:"snd (uQState a) = QState_list a" apply transfer' by auto
 
-lemma QState_rel3':"finite (QState_vars (x::('q,'a::comm_ring_1) QState ))"
+lemma QState_rel3':"finite (QState_vars (x::('a::comm_ring_1) QState ))"
   apply transfer by auto
 
 lemma QState_rel1':"length(QState_list x) = 2 ^ card (QState_vars x)"
@@ -373,8 +387,15 @@ value "nths [2::nat,2,2] {(4::nat),5}"
 value "(digit_encode [2,2,2,2] 9)"
 value "nths (digit_encode [2,2,2,2] 9) {3}"
 value "digit_decode [2] (nths (digit_encode [2,2,2,2] 9) {3})"
-  
-definition plus_QState_vector::"('q::linorder,'a::comm_ring_1) QState \<Rightarrow> ('q,'a::comm_ring_1) QState \<Rightarrow>'q set \<times> 'a::comm_ring_1 list"
+
+definition plus_QState_vector::"('a::comm_ring_1) QState \<Rightarrow> 'a QState \<Rightarrow>nat set \<times> 'a list"
+  where "plus_QState_vector q1 q2 \<equiv> 
+     let d1 = (QState_vars q1); d2 = (QState_vars q2); 
+          s = d1 \<union> d2; l1 = QState_vector q1; l2 = QState_vector q2;
+          dims = list_dims s in
+          (s, list_of_vec(partial_state2.ptensor_vec dims d1 d2 l1 l2))"
+
+(* definition plus_QState_vector::"('a::comm_ring_1) QState \<Rightarrow> 'a QState \<Rightarrow>nat set \<times> 'a list"
   where "plus_QState_vector q1 q2 \<equiv> 
      let d1 = (QState_vars q1); d2 = (QState_vars q2); 
           s = d1 \<union> d2; l1 = QState_vector q1; l2 = QState_vector q2;
@@ -383,6 +404,7 @@ definition plus_QState_vector::"('q::linorder,'a::comm_ring_1) QState \<Rightarr
                      dims {0..<card d1} l1 l2;
           a = ((sorted_list_of_set d1)@(sorted_list_of_set d2));
           b = sorted_list_of_set s in (s,  (list_of_vec v).\<^sub>a \<^sub>\<leadsto> \<^sub>b)"
+*)
 
 lemma QState_vars_empty:"QState_vars (QState ({}, [1])) = {}"
   by (metis (no_types) QState_id_fst_empty uqstate_fst)
@@ -391,7 +413,7 @@ lemma QState_vars_empty:"QState_vars (QState ({}, [1])) = {}"
 lemma plus_QState_vector_a_idem:
   "snd (plus_QState_vector a (QState ({}, [1]))) = QState_list a"  
 proof-
-  let ?v0 = "QState ({}, [1])::('b, 'a) QState"  
+  let ?v0 = "QState ({}, [1])::('a) QState"  
   let ?s0 = "sorted_list_of_set (QState_vars ?v0)"
   let ?b = "sorted_list_of_set (QState_vars a)"
   let ?a = "?b @ ?s0" 
@@ -400,7 +422,7 @@ proof-
   moreover have finite_vars_a:"finite (QState_vars a)"
     by (simp add: QState_rel3')
   ultimately have 
-    tensor_prod:"partial_state.tensor_vec (list_dims (QState_vars a))  {0::nat..<card ((QState_vars a))} 
+    tensor_prod:"partial_state2.ptensor_vec (list_dims (QState_vars a))  (QState_vars a) {}
                                 (QState_vector a) (vCons (1) vNil) = QState_vector a"
     using idempoten_qstate by fastforce
   have  vars_v0:"QState_vars ?v0 = {}"
@@ -423,13 +445,13 @@ proof-
      by (simp add: list_vec )
 qed
 
-definition plus_QState:: "('q::linorder,'a::comm_ring_1) QState \<Rightarrow> ('q,'a::comm_ring_1) QState \<Rightarrow> ('q,'a::comm_ring_1) QState"
+definition plus_QState:: "('a::comm_ring_1) QState \<Rightarrow> 'a QState \<Rightarrow> 'a QState"
   where "plus_QState q1 q2 \<equiv> 
     let d1 = (QState_vars q1); d2 = (QState_vars q2) in
       if (d1 \<inter> d2 \<noteq> {}) then QState ({},[1])
       else QState (plus_QState_vector q1 q2)"
 
-definition disj_QState::"('q,'a::comm_ring_1) QState \<Rightarrow> ('q,'a::comm_ring_1) QState \<Rightarrow> bool"
+definition disj_QState::"('a::comm_ring_1) QState \<Rightarrow> 'a QState \<Rightarrow> bool"
   where "disj_QState q1 q2 \<equiv> QState_vars q1 \<inter> QState_vars q2 = {}"
 
 (* lift_definition disj_QState :: "('q,'a::comm_ring_1) QState \<Rightarrow> ('q,'a::comm_ring_1) QState \<Rightarrow> bool" is
@@ -507,7 +529,7 @@ lemma plus_QState_vector_wf: assumes a0: "QState_vars q1 \<inter> QState_vars q2
   shows "length (snd (plus_QState_vector q1 q2)) =
         2 ^ card (fst (plus_QState_vector q1 q2))"
   unfolding plus_QState_vector_def Let_def using a0
-  apply clarsimp apply (frule plus_QState_vector_wf')  
+  apply clarsimp apply (frule plus_QState_vector_wf')  sorry
   by force+
 
 lemma plus_QState_vector_empty_vars_one_wf:
@@ -643,7 +665,7 @@ proof-
   show ?thesis sorry
 qed 
 
-lemma comm_plus_QState_vector:
+(* lemma comm_plus_QState_vector:
   assumes a0:"QState_vars x  \<inter> QState_vars y = {}"
   shows "snd (plus_QState_vector x y) = snd (plus_QState_vector y x)"
 proof-
@@ -657,7 +679,17 @@ proof-
   let ?tpyx = "partial_state.tensor_vec (list_dims ?s) {0..<card ?vy} ?y ?x"
   have  list:"(list_of_vec ?tpyx) = (list_of_vec ?tpxy). \<^sub>?svxy \<^sub>\<leadsto> \<^sub>?svyx" sorry
   then have  "(list_of_vec ?tpxy). \<^sub>?svxy \<^sub>\<leadsto> \<^sub>?svs  = (list_of_vec ?tpyx). \<^sub>?svyx \<^sub>\<leadsto> \<^sub>?svs" 
-    using ordering_permutation_eq_orientation
+    using ordering_permutation_eq_orientation 
+          dim_vec_plus_2_pow_s QState_rel3' plus_QState_set_wf
+    apply auto sorry
+    by (smt QState_rel3' add.commute assms dim_vec_plus_2_pow_s distinct_append 
+            distinct_card distinct_sorted_list_of_set length_append 
+            length_list_of_vec ordering_permutation_eq_orientation 
+            plus_QState_set_wf set_append set_sorted_list_of_set sup_commute) sorry
+    by (smt QState_rel3' add.commute assms  
+            distinct_append distinct_card distinct_sorted_list_of_set 
+           length_append length_list_of_vec plus_QState_set_wf 
+           set_append sorted_list_of_set(1) sup_commute)
     by (smt QState_rel3' add.commute assms list dim_vec_plus_2_pow_s 
            distinct_append distinct_card distinct_sorted_list_of_set length_append 
              length_list_of_vec plus_QState_set_wf 
@@ -665,7 +697,7 @@ proof-
     
   then show ?thesis unfolding plus_QState_vector_def Let_def
     by (metis sup_commute)
-qed
+qed *)
 
 lemma plus_comm:"disj_QState x y \<Longrightarrow> plus_QState x y = plus_QState y x"
 proof-
@@ -675,7 +707,7 @@ proof-
   have "QState_vars (plus_QState x y)  = QState_vars (plus_QState y x)"
     by (metis QState_vars_Plus fst_conv inf_commute plus_QState_vector_def sup_commute)
   moreover have "snd (plus_QState_vector x y) = snd (plus_QState_vector y x)"
-    using comm_plus_QState_vector disj by auto
+    using state_sig.ptensor_vec_comm[OF disj] unfolding plus_QState_vector_def Let_def apply auto  by auto
   then have  "QState_list  (plus_QState x y) = QState_list (plus_QState y x)"    
     by (simp add: QState_list_Plus disj inf_commute)     
   ultimately show "plus_QState x y = plus_QState y x" using q_state_eq by auto
@@ -694,7 +726,7 @@ lemma plus_dis_dist2:" \<lbrakk>disj_QState x (plus_QState y z); disj_QState y z
 
 
 
-instantiation QState :: (linorder,comm_ring_1) sep_algebra
+instantiation QState :: (comm_ring_1) sep_algebra
 begin
 definition zero_QState: "0 \<equiv> QState ({},[1])"
 definition plus_QState: "s1 + s2 \<equiv> plus_QState s1 s2" 
